cfrontend/Clight.v
@@ -573,14 +573,15 @@ Inductive step: state -> trace -> state -> Prop :=
       Genv.find_funct ge vf = Some fd ->
       type_of_fundef fd = Tfunction tyargs tyres cconv ->
       step (State f (Scall optid a al) k e le m)
-        E0 (Callstate fd vargs (Kcall optid f e le k) m (fn_stack_requirements id))
+        E0 (Callstate fd vargs (Kcall optid f e le k) (Mem.push_new_stage m) (fn_stack_requirements id))
 
-  | step_builtin:   forall f optid ef tyargs al k e le m vargs t vres m',
+  | step_builtin:   forall f optid ef tyargs al k e le m vargs t vres m' m'',
       eval_exprlist e le m al tyargs vargs ->
-      external_call ef ge vargs m t vres m' ->
+      external_call ef ge vargs (Mem.push_new_stage m) t vres m' ->
+      Mem.unrecord_stack_block m' = Some m'' ->
       forall BUILTIN_ENABLED: builtin_enabled ef,
       step (State f (Sbuiltin optid ef tyargs al) k e le m)
-         t (State f Sskip k e (set_opttemp optid vres le) m')
+         t (State f Sskip k e (set_opttemp optid vres le) m'')
 
   | step_seq:  forall f s1 s2 k e le m,
       step (State f (Ssequence s1 s2) k e le m)
@@ -618,24 +619,21 @@ Inductive step: state -> trace -> state -> Prop :=
       step (State f Sbreak (Kloop2 s1 s2 k) e le m)
         E0 (State f Sskip k e le m)
 
-  | step_return_0: forall f k e le m m' m'',
+  | step_return_0: forall f k e le m m',
       Mem.free_list m (blocks_of_env e) = Some m' ->
-      Mem.unrecord_stack_block m' = Some m'' ->
       step (State f (Sreturn None) k e le m)
-        E0 (Returnstate Vundef (call_cont k) m'')
-  | step_return_1: forall f a k e le m v v' m' m'',
+        E0 (Returnstate Vundef (call_cont k) m')
+  | step_return_1: forall f a k e le m v v' m',
       eval_expr e le m a v ->
       sem_cast v (typeof a) f.(fn_return) m = Some v' ->
       Mem.free_list m (blocks_of_env e) = Some m' ->
-      Mem.unrecord_stack_block m' = Some m'' ->
       step (State f (Sreturn (Some a)) k e le m)
-        E0 (Returnstate v' (call_cont k) m'')
-  | step_skip_call: forall f k e le m m' m'',
+        E0 (Returnstate v' (call_cont k) m')
+  | step_skip_call: forall f k e le m m',
       is_call_cont k ->
       Mem.free_list m (blocks_of_env e) = Some m' ->
-      Mem.unrecord_stack_block m' = Some m'' ->
       step (State f Sskip k e le m)
-        E0 (Returnstate Vundef k m'')
+        E0 (Returnstate Vundef k m')
 
   | step_switch: forall f a sl k e le m v n,
       eval_expr e le m a v ->
@@ -669,9 +667,10 @@ Inductive step: state -> trace -> state -> Prop :=
       step (Callstate (External ef targs tres cconv) vargs k m sz)
          t (Returnstate vres k m')
 
-  | step_returnstate: forall v optid f e le k m,
+  | step_returnstate: forall v optid f e le k m m',
+      Mem.unrecord_stack_block m = Some m' ->
       step (Returnstate v (Kcall optid f e le k) m)
-        E0 (State f Sskip k e (set_opttemp optid v le) m).
+        E0 (State f Sskip k e (set_opttemp optid v le) m').
 
 (** ** Whole-program semantics *)
 
@@ -689,7 +688,7 @@ Inductive initial_state (p: program): state -> Prop :=
       type_of_fundef f = Tfunction Tnil type_int32s cc_default ->
       Mem.alloc m0 0 0 = (m1,b1) ->
       Mem.record_stack_blocks (Mem.push_new_stage m1) (make_singleton_frame_adt b1 0 0) = Some m2 ->
-      initial_state p (Callstate f nil Kstop m2 (fn_stack_requirements (prog_main p))).
+      initial_state p (Callstate f nil Kstop (Mem.push_new_stage m2) (fn_stack_requirements (prog_main p))).
 
 (** A final state is a [Returnstate] with an empty continuation. *)
 
@@ -756,6 +755,8 @@ Proof.
   inversion H; subst; auto.
   (* builtin *)
   exploit external_call_receptive; eauto. intros [vres2 [m2 EC2]].
+  edestruct (Mem.unrecord_stack_block_succeeds m2) as (m2' & USB & EQ).
+  repeat rewrite_stack_blocks; reflexivity.
   econstructor; econstructor; eauto.
   (* external *)
   exploit external_call_receptive; eauto. intros [vres2 [m2 EC2]].
